Adjust BMV_Fixpoint operations theory for sealed mrsbnf

operations/BMV_Fixpoint.thy
@@ -29,6 +29,14 @@ let
 
   val mrsbnf = case mrsbnf of MRBNF_Util.Inl x => x | _ => error "impossible"
 
+  val notes = [
+      ("bmv_defs", bmv_unfolds)
+    ] |> (map (fn (thmN, thms) =>
+      ((Binding.name thmN, []), [(thms, [])])
+    ));
+
+    val (noted, lthy) = Local_Theory.notes notes lthy
+
   val ((mrsbnf, (tys, info)), lthy) = MRSBNF_Comp.seal_mrsbnf I (bmv_unfolds, mrbnf_unfolds)
     @{binding FTerm_pre} Xs Ds mrsbnf NONE lthy
   val (_, lthy) = MRSBNF_Def.note_mrsbnf_thms (K BNF_Def.Note_Some) I NONE mrsbnf lthy
@@ -39,15 +47,18 @@ let
   (* Step 3: Register the pre-MRBNF as a BNF in its live variables *)
     val (bnf, lthy) = MRBNF_Def.register_mrbnf_as_bnf mrbnf lthy
 
-    (* Step 4: Construct the binder fixpoint *)
-    val (fp_res, lthy) = MRBNF_FP.construct_binder_fp BNF_Util.Least_FP
-    [{
-      FVars = [SOME "FTVars", SOME "FVars"],
-      T_name = "FTerm",
-      nrecs = 2,
-      permute = NONE,
-      pre_mrbnf = mrbnf
-    }] [[([], [0])], [([], [0])]] lthy
+  (* Step 4: Construct the binder fixpoint *)
+  val (fp_res, lthy) = MRBNF_FP.construct_binder_fp BNF_Util.Least_FP
+  [{
+    FVars = [SOME "FTVars", SOME "FVars"],
+    T_name = "FTerm",
+    nrecs = 2,
+    permute = NONE,
+    pre_mrbnf = mrbnf
+  }] [[([], [0])], [([], [0])]] lthy
+
+  (* Step 5: Define recursor locales *)  
+  val (recursor_result, lthy) = MRBNF_Recursor.create_binding_recursor I fp_res lthy;
 
 in lthy end
 \<close>
@@ -78,8 +89,6 @@ lemma eta_natural:
   done
 
 (* Construction of substitution *)
-type_synonym ('tv, 'v) P = "('v \<Rightarrow> ('tv, 'v) FTerm) \<times> ('tv \<Rightarrow> 'tv FType)"
-
 definition VVr :: "'v::var \<Rightarrow> ('tv::var, 'v) FTerm" where
   "VVr \<equiv> FTerm_ctor \<circ> \<eta>"
 definition isVVr :: "('tv::var, 'v::var) FTerm \<Rightarrow> bool" where
@@ -87,37 +96,8 @@ definition isVVr :: "('tv::var, 'v::var) FTerm \<Rightarrow> bool" where
 definition asVVr :: "('tv::var, 'v::var) FTerm \<Rightarrow> 'v" where
   "asVVr x \<equiv> (if isVVr x then SOME a. x = VVr a else undefined)"
 
-definition SSupp_FTerm :: "('v \<Rightarrow> ('tv::var, 'v::var) FTerm) \<Rightarrow> 'v set" where
-  "SSupp_FTerm f \<equiv> { a. f a \<noteq> VVr a }"
-definition IImsupp_FTerm1 :: "('v \<Rightarrow> ('tv::var, 'v::var) FTerm) \<Rightarrow> 'tv set" where
-  "IImsupp_FTerm1 f \<equiv> \<Union>(FTVars ` f ` SSupp_FTerm f)"
-definition IImsupp_FTerm2 :: "('v \<Rightarrow> ('tv::var, 'v::var) FTerm) \<Rightarrow> 'v set" where
-  "IImsupp_FTerm2 f \<equiv> SSupp_FTerm f \<union> \<Union>(FVars ` f ` SSupp_FTerm f)"
-
-definition Uctor :: "('tv::var, 'v::var, 'tv, 'v, ('tv, 'v) FTerm \<times> (('tv, 'v) P \<Rightarrow> ('tv, 'v) FTerm), ('tv, 'v) FTerm \<times> (('tv, 'v) P \<Rightarrow> ('tv, 'v) FTerm)) FTerm_pre
-  \<Rightarrow> ('tv, 'v) P \<Rightarrow> ('tv, 'v) FTerm" where
-  "Uctor y p \<equiv> case p of (f1, f2) \<Rightarrow> if isVVr (FTerm_ctor (map_FTerm_pre id id id id fst fst y)) then
-    f1 (asVVr (FTerm_ctor (map_FTerm_pre id id id id fst fst y)))
-  else
-    FTerm_ctor (Sb_FTerm_pre id f2 (map_FTerm_pre id id id id ((\<lambda>R. R (f1, f2)) \<circ> snd) ((\<lambda>R. R (f1, f2)) \<circ> snd) y))"
-
-definition PFVars_1 :: "('tv::var, 'v::var) P \<Rightarrow> 'tv set" where
-  "PFVars_1 p \<equiv> case p of (f1, f2) \<Rightarrow> IImsupp_FTerm1 f1 \<union> IImsupp_FType f2"
-definition PFVars_2 :: "('tv::var, 'v::var) P \<Rightarrow> 'v set" where
-  "PFVars_2 p \<equiv> case p of (f1, _) \<Rightarrow> IImsupp_FTerm2 f1"
-
-definition compSS_FType :: "('tv \<Rightarrow> 'tv) \<Rightarrow> ('tv \<Rightarrow> 'tv::var FType) \<Rightarrow> 'tv \<Rightarrow> 'tv FType" where
-  "compSS_FType g f \<equiv> permute_FType g \<circ> f \<circ> inv g"
-definition compSS_FTerm :: "('tv \<Rightarrow> 'tv) \<Rightarrow> ('v \<Rightarrow> 'v) \<Rightarrow> ('v \<Rightarrow> ('tv::var, 'v::var) FTerm) \<Rightarrow> 'v \<Rightarrow> ('tv, 'v) FTerm" where
-  "compSS_FTerm g1 g2 f \<equiv> permute_FTerm g1 g2 \<circ> f \<circ> inv g2"
-definition Pmap :: "('tv \<Rightarrow> 'tv) \<Rightarrow> ('v \<Rightarrow> 'v) \<Rightarrow> ('tv::var, 'v::var) P \<Rightarrow> ('tv, 'v) P" where
-  "Pmap g1 g2 p \<equiv> case p of (f1, f2) \<Rightarrow> (compSS_FTerm g1 g2 f1, compSS_FType g1 f2)"
-lemmas compSS_defs = compSS_FType_def compSS_FTerm_def
-
-definition valid_P :: "('tv::var, 'v::var) P \<Rightarrow> bool" where
-  "valid_P p \<equiv> case p of (f1, f2) \<Rightarrow>
-    |SSupp_FTerm f1| <o cmin |UNIV::'tv set| |UNIV::'v set|
-  \<and> |SSupp_FType f2| <o cmin |UNIV::'tv set| |UNIV::'v set|"
+abbreviation "IImsupp_FTerm1 \<equiv> IImsupp VVr FTVars"
+abbreviation "IImsupp_FTerm2 f \<equiv> SSupp VVr f \<union> IImsupp VVr FVars f"
 
 lemma asVVr_VVr: "asVVr (VVr a) = a"
   apply (unfold asVVr_def isVVr_def)
@@ -173,31 +153,8 @@ lemma isVVr_permute:
   apply (rule refl)
   done
 
-lemma compSS_id0s:
-  "compSS_FType id = id"
-  "compSS_FTerm id id = id"
-  apply (unfold compSS_FType_def compSS_FTerm_def FTerm.permute_id0 FType.permute_id0 id_o o_id inv_id)
-  apply (unfold id_def)
-  apply (rule refl)+
-  done
-
-lemma compSS_comp0_FTerm:
-  fixes f1 g1::"'tyvar::var \<Rightarrow> 'tyvar" and f2 g2::"'var::var \<Rightarrow> 'var"
-  assumes g_prems: "bij g1" "|supp g1| <o cmin |UNIV::'tyvar set| |UNIV::'var set|" "bij g2" "|supp g2| <o cmin |UNIV::'tyvar set| |UNIV::'var set|"
-    and f_prems: "bij f1" "|supp f1| <o cmin |UNIV::'tyvar set| |UNIV::'var set|" "bij f2" "|supp f2| <o cmin |UNIV::'tyvar set| |UNIV::'var set|"
-  shows
-    "compSS_FTerm f1 f2 \<circ> compSS_FTerm g1 g2 = compSS_FTerm (f1 \<circ> g1) (f2 \<circ> g2)"
-  apply (unfold compSS_FTerm_def)
-  apply (subst o_inv_distrib FTerm.permute_comp0[symmetric], (rule supp_id_bound bij_id assms ordLess_ordLeq_trans cmin2 cmin1 card_of_Card_order)+)+
-  apply (rule ext)
-  apply (rule trans[OF comp_apply])
-  apply (unfold comp_assoc)
-  apply (rule refl)
-  done
-lemmas compSS_comp0s = FType.compSS_comp0[unfolded tvcompSS_tvsubst_FType_def compSS_FType_def[symmetric]] compSS_comp0_FTerm
-
 lemma IImsupp_VVrs: "f2 a \<noteq> a \<Longrightarrow> imsupp f2 \<inter> IImsupp_FTerm2 y = {} \<Longrightarrow> y a = VVr a"
-  apply (unfold imsupp_def supp_def IImsupp_FTerm2_def SSupp_FTerm_def)
+  apply (unfold imsupp_def supp_def SSupp_def)
   apply (drule iffD1[OF disjoint_iff])
   apply (erule allE)
   apply (erule impE)
@@ -238,12 +195,11 @@ lemma IImsupp_permute_commute:
        apply (erule id_onD[rotated])
        apply (rule imsupp_id_on)
        apply (erule Int_subset_empty2)
-       apply (unfold IImsupp_FTerm1_def SSupp_FTerm_def)[1]
+       apply (unfold SSupp_def IImsupp_def)[1]
        apply (rule subsetI)
        apply (rule UnI2)?
        apply (rule UN_I[rotated])
         apply assumption
-       apply (rule imageI)
        apply (rule CollectI)
        apply assumption
       (* repeated *)
@@ -251,12 +207,11 @@ lemma IImsupp_permute_commute:
       apply (erule id_onD[rotated])
       apply (rule imsupp_id_on)
       apply (erule Int_subset_empty2)
-      apply (unfold IImsupp_FTerm2_def SSupp_FTerm_def)[1]
+       apply (unfold SSupp_def IImsupp_def)[1]
       apply (rule subsetI)
       apply (rule UnI2)?
       apply (rule UN_I[rotated])
        apply assumption
-      apply (rule imageI)
       apply (rule CollectI)
       apply assumption
       (* END REPEAT_DETERM *)
@@ -281,38 +236,7 @@ lemma IImsupp_permute_commute:
     done
   done
 
-lemma compSS_cong_id_FTerm:
-  fixes f1 g1::"'tyvar::var \<Rightarrow> 'tyvar" and f2 g2::"'var::var \<Rightarrow> 'var"
-  assumes g_prems: "bij g1" "|supp g1| <o cmin |UNIV::'tyvar set| |UNIV::'var set|" "bij g2" "|supp g2| <o cmin |UNIV::'tyvar set| |UNIV::'var set|"
-    and f_prems: "bij f1" "|supp f1| <o cmin |UNIV::'tyvar set| |UNIV::'var set|" "bij f2" "|supp f2| <o cmin |UNIV::'tyvar set| |UNIV::'var set|"
-  shows
-    "(\<And>a. a \<in> IImsupp_FTerm1 h \<Longrightarrow> f1 a = a) \<Longrightarrow> (\<And>a. a \<in> IImsupp_FTerm2 h \<Longrightarrow> f2 a = a) \<Longrightarrow> compSS_FTerm f1 f2 h = h"
-  apply (unfold compSS_FTerm_def)
-  subgoal premises prems
-    apply (subst IImsupp_permute_commute)
-          apply (rule assms cmin1 cmin2 card_of_Card_order ordLess_ordLeq_trans)+
-    (* REPEAT_DETERM *)
-      apply (rule trans[OF Int_commute])
-      apply (rule disjointI)
-      apply (drule prems)
-      apply (erule bij_id_imsupp[rotated])
-      apply (rule assms)
-    (* repeated *)
-      apply (rule trans[OF Int_commute])
-      apply (rule disjointI)
-      apply (drule prems)
-      apply (erule bij_id_imsupp[rotated])
-      apply (rule assms)
-    (* END REPEAT_DETERM *)
-    apply (unfold comp_assoc)
-    apply (subst inv_o_simp2)
-     apply (rule assms)
-    apply (rule o_id)
-    done
-  done
-lemmas compSS_cong_ids = FType.compSS_cong_id[unfolded tvcompSS_tvsubst_FType_def compSS_FType_def[symmetric]] compSS_cong_id_FTerm
-
-lemma SSupp_natural_FTerm:
+(*lemma SSupp_natural_FTerm:
   fixes f1::"'tyvar::var \<Rightarrow> 'tyvar" and f2::"'var::var \<Rightarrow> 'var"
   assumes f_prems: "bij f1" "|supp f1| <o |UNIV::'tyvar set|" "bij f2" "|supp f2| <o |UNIV::'var set|"
   shows
@@ -397,404 +321,7 @@ lemma IImsupp_natural_FTerm:
   apply (rule refl)
   done
 lemmas IImsupp_naturals = FType.IImsupp_natural IImsupp_natural_FTerm
-
-(* Recursor axioms *)
-lemma Pmap_id0: "Pmap id id = id"
-  apply (rule ext)
-  apply (unfold Pmap_def case_prod_beta compSS_id0s)
-  apply (unfold id_def prod.collapse)
-  apply (rule refl)
-  done
-
-lemma Pmap_comp0:
-  fixes f1 g1::"'tyvar::var \<Rightarrow> 'tyvar" and f2 g2::"'var::var \<Rightarrow> 'var"
-  assumes g_prems: "bij g1" "|supp g1| <o cmin |UNIV::'tyvar set| |UNIV::'var set|" "bij g2" "|supp g2| <o cmin |UNIV::'tyvar set| |UNIV::'var set|"
-    and f_prems: "bij f1" "|supp f1| <o cmin |UNIV::'tyvar set| |UNIV::'var set|" "bij f2" "|supp f2| <o cmin |UNIV::'tyvar set| |UNIV::'var set|"
-  shows
-    "Pmap f1 f2 \<circ> Pmap g1 g2 = Pmap (f1 \<circ> g1) (f2 \<circ> g2)"
-  apply (rule ext)
-  apply (unfold Pmap_def case_prod_beta)
-  apply (rule trans[OF comp_apply])
-  apply (unfold prod.inject fst_conv snd_conv)
-  apply (rule conjI bij_id supp_id_bound assms ordLess_ordLeq_trans cmin1 card_of_Card_order
-      trans[OF comp_apply[symmetric] fun_cong[OF compSS_comp0s(1)]]
-      trans[OF comp_apply[symmetric] fun_cong[OF compSS_comp0s(2)]]
-      )+
-  done
-
-lemma valid_Pmap:
-  fixes f1::"'tyvar::var \<Rightarrow> 'tyvar" and f2::"'var::var \<Rightarrow> 'var"
-  assumes f_prems: "bij f1" "|supp f1| <o cmin |UNIV::'tyvar set| |UNIV::'var set|" "bij f2" "|supp f2| <o cmin |UNIV::'tyvar set| |UNIV::'var set|"
-  shows "valid_P p \<Longrightarrow> valid_P (Pmap f1 f2 p)"
-  apply (unfold valid_P_def Pmap_def case_prod_beta compSS_defs fst_conv snd_conv)
-  apply (erule conj_forward)+
-   apply (subst SSupp_naturals; (assumption | rule assms cmin1 cmin2 card_of_Card_order ordLeq_ordLess_trans[OF card_of_image] ordLess_ordLeq_trans)+)+
-  done
-
-lemma PFVars_Pmaps:
-  fixes f1::"'tyvar::var \<Rightarrow> 'tyvar" and f2::"'var::var \<Rightarrow> 'var"
-  assumes f_prems: "bij f1" "|supp f1| <o cmin |UNIV::'tyvar set| |UNIV::'var set|" "bij f2" "|supp f2| <o cmin |UNIV::'tyvar set| |UNIV::'var set|"
-  shows "PFVars_1 (Pmap f1 f2 p) = f1 ` PFVars_1 p"
-    "PFVars_2 (Pmap f1 f2 p) = f2 ` PFVars_2 p"
-  subgoal
-    apply (unfold PFVars_1_def Pmap_def case_prod_beta fst_conv snd_conv compSS_defs)
-    apply (subst IImsupp_naturals, (rule assms cmin1 cmin2 card_of_Card_order ordLess_ordLeq_trans)+)+
-    apply (unfold image_Un)?
-    apply (rule refl)
-    done
-  subgoal
-    apply (unfold PFVars_2_def Pmap_def case_prod_beta fst_conv snd_conv compSS_defs)
-    apply (subst IImsupp_naturals, (rule assms cmin1 cmin2 card_of_Card_order ordLess_ordLeq_trans)+)+
-    apply (unfold image_Un)?
-    apply (rule refl)
-    done
-  done
-
-lemma Pmap_cong_id:
-  fixes f1::"'tyvar::var \<Rightarrow> 'tyvar" and f2::"'var::var \<Rightarrow> 'var"
-  assumes f_prems: "bij f1" "|supp f1| <o cmin |UNIV::'tyvar set| |UNIV::'var set|" "bij f2" "|supp f2| <o cmin |UNIV::'tyvar set| |UNIV::'var set|"
-  shows "(\<And>a. a \<in> PFVars_1 p \<Longrightarrow> f1 a = a) \<Longrightarrow> (\<And>a. a \<in> PFVars_2 p \<Longrightarrow> f2 a = a) \<Longrightarrow> Pmap f1 f2 p = p"
-  apply (unfold PFVars_1_def PFVars_2_def Pmap_def case_prod_beta)
-  subgoal premises prems
-    apply (subst compSS_cong_ids, (rule f_prems prems cmin1 cmin2 card_of_Card_order ordLess_ordLeq_trans | erule UnI2 UnI1 | rule UnI1)+)+
-    apply assumption
-    apply (unfold prod.collapse)
-    apply (rule refl)
-    done
-  done
-
-lemmas Cinfinite_UNIV = conjI[OF FTerm_pre.UNIV_cinfinite card_of_Card_order]
-lemmas Cinfinite_card = cmin_Cinfinite[OF Cinfinite_UNIV Cinfinite_UNIV]
-lemmas regularCard_card = cmin_regularCard[OF FTerm_pre.var_regular FTerm_pre.var_regular Cinfinite_UNIV Cinfinite_UNIV]
-lemmas Un_bound = regularCard_Un[OF conjunct2[OF Cinfinite_card] conjunct1[OF Cinfinite_card] regularCard_card]
-lemmas UN_bound = regularCard_UNION[OF conjunct2[OF Cinfinite_card] conjunct1[OF Cinfinite_card] regularCard_card]
-
-lemma small_PFVarss:
-  "valid_P p \<Longrightarrow> |PFVars_1 (p::('tyvar::var, 'var::var) P)| <o cmin |UNIV::'tyvar set| |UNIV::'var set|"
-  "valid_P p \<Longrightarrow> |PFVars_2 p| <o cmin |UNIV::'tyvar set| |UNIV::'var set|"
-  subgoal
-    apply (unfold PFVars_1_def case_prod_beta IImsupp_FTerm1_def IImsupp_FTerm2_def IImsupp_FType_def comp_def valid_P_def)
-    apply (erule conjE)+
-        apply (assumption | rule Un_bound UN_bound ordLeq_ordLess_trans[OF card_of_image] FType.set_bd_UNIV FTerm.FVars_bd_UNIVs cmin_greater card_of_Card_order)+
-    done
-  (* copied from above *)
-  subgoal
-    apply (unfold PFVars_2_def case_prod_beta IImsupp_FTerm1_def IImsupp_FTerm2_def IImsupp_FType_def comp_def valid_P_def)
-    apply (erule conjE)+
-        apply (assumption | rule Un_bound UN_bound ordLeq_ordLess_trans[OF card_of_image] FType.set_bd_UNIV FTerm.FVars_bd_UNIVs cmin_greater card_of_Card_order)+
-    done
-  done
-
-lemma FTVars_subset: "valid_P p \<Longrightarrow> set3_FTerm_pre y \<inter> PFVars_1 p = {} \<Longrightarrow>
-  (\<And>t pu p. valid_P p \<Longrightarrow> (t, pu) \<in> set5_FTerm_pre y \<union> set6_FTerm_pre y \<Longrightarrow> FTVars (pu p) \<subseteq> FTVars t \<union> PFVars_1 p) \<Longrightarrow>
-  FTVars (Uctor y p) \<subseteq> FTVars (FTerm_ctor (map_FTerm_pre id id id id fst fst y)) \<union> PFVars_1 p"
-  apply (frule iffD1[OF meta_eq_to_obj_eq[OF valid_P_def]])
-  apply (unfold case_prod_beta)
-  apply (erule conjE)+
-  subgoal premises prems
-    apply (unfold Uctor_def case_prod_beta)
-    apply (rule case_split)
-     apply (subst if_P)
-      apply assumption
-     apply (unfold isVVr_def)[1]
-     apply (erule exE)
-     apply (drule sym)
-    apply (erule subst)
-     apply (unfold asVVr_VVr)
-     apply (rule case_split[of "_ = _"])
-      apply (rule iffD2[OF arg_cong2[OF _ refl, of _ _ "(\<subseteq>)"]])
-       apply (rule arg_cong[of _ _ FTVars])
-       apply assumption
-      apply (rule Un_upper1)
-     apply (rule subsetI)
-     apply (rule UnI2)
-     apply (unfold PFVars_1_def case_prod_beta IImsupp_FTerm1_def SSupp_FTerm_def image_comp[unfolded comp_def])[1]
-     apply (rule UnI1)
-     apply (rule UN_I)
-      apply (rule CollectI)
-      apply assumption
-     apply assumption
-    apply (unfold if_not_P)
-    apply (erule thin_rl)
-
-    apply (tactic \<open>EqSubst.eqsubst_tac @{context} [0] [Map_Sb'] 1\<close>)
-      apply (rule FTerm_pre.SSupp_Inj_bound prems(4,5)[THEN ordLess_ordLeq_trans] cmin1 cmin2 card_of_Card_order)+
-
-    apply (unfold FTerm.FVars_ctor prod.collapse)
-    apply (subst FTerm_pre.set_map, (rule bij_id supp_id_bound)+)+
-    apply (unfold image_id image_comp comp_def prod.collapse)
-    apply (rule Un_mono')+
-      apply (unfold FTerm_pre.set_Sb FTerm_pre.set_Vrs)
-      apply (tactic \<open>EqSubst.eqsubst_tac @{context} [0] Vrs_Sb 1\<close>)
-        apply (rule FTerm_pre.SSupp_Inj_bound prems(4,5)[THEN ordLess_ordLeq_trans] cmin1 cmin2 card_of_Card_order)+
-      apply (unfold PFVars_1_def case_prod_beta IImsupp_FType_def SSupp_FType_def
-        tvVVr_tvsubst_FType_def tv\<eta>_FType_tvsubst_FType_def TyVar_def[symmetric] comp_def
-      )[1]
-      apply (rule subsetI)
-      apply (erule UN_E)
-    apply (rule case_split[of "_ = _", rotated])
-      apply (rule UnI2)+
-       apply (rule UN_I)
-        apply (rule CollectI)
-        apply assumption
-       apply assumption
-      apply (rule UnI1)
-      apply (rotate_tac -2)
-      apply (drule iffD1[OF arg_cong2[OF refl, of _ _ "(\<in>)"], rotated])
-       apply (erule arg_cong)
-      apply (tactic \<open>Local_Defs.unfold0_tac @{context} Vrs_Injs\<close>)
-      apply (drule singletonD)
-      apply hypsubst
-      apply assumption
-
-     apply (subst FTerm_pre.set_Sb)
-      apply (rule FTerm_pre.SSupp_Inj_bound prems(4,5)[THEN ordLess_ordLeq_trans] cmin1 cmin2 card_of_Card_order)+
-    apply (rule iffD2[OF arg_cong2[OF refl, of _ _ "(\<subseteq>)"]])
-      apply (rule Diff_Un_disjunct)
-      apply (rule prems)
-     apply (rule Diff_mono[OF _ subset_refl])
-     apply (unfold UN_extend_simps(2))
-    (* REPEAT_DETERM *)
-     apply (rule subset_If)
-      apply (tactic \<open>Local_Defs.unfold0_tac @{context} (#Supp_Sb param)\<close>)
-      apply (unfold UN_empty')[1]
-      apply (rule empty_subsetI)
-     apply (rule UN_mono[OF subset_refl])
-     apply (rule prems)
-      apply (rule prems)
-     apply (unfold prod.collapse)
-     apply (erule UnI2 UnI1)
-    (* repeated *)
-     apply (rule subset_If)
-      apply (tactic \<open>Local_Defs.unfold0_tac @{context} (#Supp_Sb param)\<close>)
-      apply (unfold UN_empty')[1]
-      apply (rule empty_subsetI)
-     apply (rule UN_mono[OF subset_refl])
-     apply (rule prems)
-      apply (rule prems)
-     apply (unfold prod.collapse)
-     apply (erule UnI2 UnI1)
-    (* END REPEAT_DETERM *)
-    done
-  done
-
-lemma FVars_subset: "valid_P p \<Longrightarrow> set4_FTerm_pre y \<inter> PFVars_2 p = {} \<Longrightarrow>
-  (\<And>t pu p. valid_P p \<Longrightarrow> (t, pu) \<in> set5_FTerm_pre y \<union> set6_FTerm_pre y \<Longrightarrow> FVars (pu p) \<subseteq> FVars t \<union> PFVars_2 p) \<Longrightarrow>
-  FVars (Uctor y p) \<subseteq> FVars (FTerm_ctor (map_FTerm_pre id id id id fst fst y)) \<union> PFVars_2 p"
-  apply (frule iffD1[OF meta_eq_to_obj_eq[OF valid_P_def]])
-  apply (unfold case_prod_beta)
-  apply (erule conjE)+
-  subgoal premises prems
-    apply (unfold Uctor_def case_prod_beta)
-    apply (rule case_split)
-     apply (subst if_P)
-      apply assumption
-     apply (unfold isVVr_def)[1]
-     apply (erule exE)
-     apply (drule sym)
-    apply (erule subst)
-     apply (unfold asVVr_VVr)
-     apply (rule case_split[of "_ = _"])
-      apply (rule iffD2[OF arg_cong2[OF _ refl, of _ _ "(\<subseteq>)"]])
-       apply (rule arg_cong[of _ _ FVars])
-       apply assumption
-      apply (rule Un_upper1)
-     apply (rule subsetI)
-     apply (rule UnI2)
-     apply (unfold PFVars_2_def case_prod_beta IImsupp_FTerm2_def SSupp_FTerm_def image_comp[unfolded comp_def])[1]
-    apply (rule UnI2)
-     apply (rule UN_I)
-      apply (rule CollectI)
-      apply assumption
-     apply assumption
-    apply (unfold if_not_P)
-    apply (erule thin_rl)
-
-    apply (tactic \<open>EqSubst.eqsubst_tac @{context} [0] [Map_Sb'] 1\<close>)
-      apply (rule FTerm_pre.SSupp_Inj_bound prems(4,5)[THEN ordLess_ordLeq_trans] cmin1 cmin2 card_of_Card_order)+
-    apply (unfold FTerm.FVars_ctor prod.collapse)
-    apply (subst FTerm_pre.set_map, (rule bij_id supp_id_bound)+)+
-    apply (unfold image_id image_comp comp_def prod.collapse)
-    apply (rule Un_mono')+
-      apply (unfold FTerm_pre.set_Vrs)
-      apply (tactic \<open>EqSubst.eqsubst_tac @{context} [0] Vrs_Sb 1\<close>)
-      apply (rule FTerm_pre.SSupp_Inj_bound prems(4,5)[THEN ordLess_ordLeq_trans] cmin1 cmin2 card_of_Card_order)+
-      apply (unfold PFVars_2_def case_prod_beta IImsupp_FTerm2_def SSupp_FType_def
-        tvVVr_tvsubst_FType_def tv\<eta>_FType_tvsubst_FType_def TyVar_def[symmetric] comp_def
-      )[1]
-      apply (rule subsetI)
-      apply (erule UN_E)
-    apply (rule UnI1)
-      apply (tactic \<open>Local_Defs.unfold0_tac @{context} Vrs_Injs\<close>)
-      apply (drule singletonD)
-      apply hypsubst
-      apply assumption
-
-     apply (subst FTerm_pre.set_Sb)
-      apply (rule FTerm_pre.SSupp_Inj_bound prems(4,5)[THEN ordLess_ordLeq_trans] cmin1 cmin2 card_of_Card_order)+
-    apply (rule iffD2[OF arg_cong2[OF refl, of _ _ "(\<subseteq>)"]])
-      apply (rule Diff_Un_disjunct)
-      apply (rule prems)
-     apply (rule Diff_mono[OF _ subset_refl])
-     apply (unfold UN_extend_simps(2))
-    (* REPEAT_DETERM *)
-     apply (rule subset_If)
-      apply (tactic \<open>Local_Defs.unfold0_tac @{context} (#Supp_Sb param)\<close>)
-      apply (unfold UN_empty')[1]
-      apply (rule empty_subsetI)
-     apply (rule UN_mono[OF subset_refl])
-     apply (rule prems)
-      apply (rule prems)
-     apply (unfold prod.collapse)
-     apply (erule UnI2 UnI1)
-    (* repeated *)
-     apply (rule subset_If)
-      apply (tactic \<open>Local_Defs.unfold0_tac @{context} (#Supp_Sb param)\<close>)
-      apply (unfold UN_empty')[1]
-      apply (rule empty_subsetI)
-     apply (rule UN_mono[OF subset_refl])
-     apply (rule prems)
-      apply (rule prems)
-     apply (unfold prod.collapse)
-     apply (erule UnI2 UnI1)
-    (* END REPEAT_DETERM *)
-    done
-  done
-
-lemma permute_Uctor:
-  fixes f1::"'tv::var \<Rightarrow> 'tv" and f2::"'v::var \<Rightarrow> 'v"
-  shows "valid_P p \<Longrightarrow> bij f1 \<Longrightarrow> |supp f1| <o cmin |UNIV::'tv set| |UNIV::'v set| \<Longrightarrow> bij f2 \<Longrightarrow> |supp f2| <o cmin |UNIV::'tv set| |UNIV::'v set|
-  \<Longrightarrow> permute_FTerm f1 f2 (Uctor y p) = Uctor (map_FTerm_pre f1 f2 f1 f2
-    (\<lambda>(t, pu). (permute_FTerm f1 f2 t, \<lambda>p. if valid_P p then permute_FTerm f1 f2 (pu (Pmap (inv f1) (inv f2) p)) else undefined))
-    (\<lambda>(t, pu). (permute_FTerm f1 f2 t, \<lambda>p. if valid_P p then permute_FTerm f1 f2 (pu (Pmap (inv f1) (inv f2) p)) else undefined))
-  y) (Pmap f1 f2 p)"
-  apply (frule iffD1[OF meta_eq_to_obj_eq[OF valid_P_def]])
-  apply (subst (asm) case_prod_beta)
-  apply (erule conjE)+
-  apply (unfold Uctor_def)
-  apply (subst FTerm_pre.map_comp, (assumption | rule supp_id_bound bij_id ordLess_ordLeq_trans cmin1 cmin2 card_of_Card_order)+)+
-  apply (unfold id_o_commute[of f1] id_o_commute[of f2] fst_o_f comp_assoc comp_def[of snd] snd_conv case_prod_beta prod.collapse)
-  apply (subst FTerm_pre.map_comp[symmetric], (assumption | rule supp_id_bound bij_id ordLess_ordLeq_trans cmin1 cmin2 card_of_Card_order)+)+
-  apply (subst FTerm.permute_ctor[symmetric] isVVr_permute, (assumption | rule ordLess_ordLeq_trans cmin1 cmin2 card_of_Card_order)+)+
-
-  apply (rule case_split)
-   apply (subst if_P)
-    apply assumption
-   apply (unfold if_P if_not_P)
-   apply (unfold isVVr_def)[1]
-   apply (erule exE)
-   apply (erule subst[OF sym])
-   apply (subst permute_VVr)
-       apply (assumption | rule ordLess_ordLeq_trans cmin1 cmin2 card_of_Card_order)+
-   apply (unfold Pmap_def case_prod_beta fst_conv snd_conv asVVr_VVr compSS_FTerm_def comp_def)[1]
-   apply (subst inv_simp1)
-    apply assumption
-   apply (rule refl)
-
-  apply (rule trans)
-   apply (rule FTerm.permute_ctor)
-      apply (assumption | rule ordLess_ordLeq_trans cmin1 cmin2 card_of_Card_order)+
-
-  apply (tactic \<open>EqSubst.eqsubst_tac @{context} [0] [Map_Sb'] 1\<close>)
-    apply (rule FTerm_pre.SSupp_Inj_bound cmin1 cmin2 card_of_Card_order
-      | erule ordLess_ordLeq_trans)+
-
-  apply (subst FTerm_pre.map_comp, (assumption | rule supp_id_bound bij_id ordLess_ordLeq_trans cmin1 cmin2 card_of_Card_order)+)+
-  apply (unfold id_o o_id)
-  apply (unfold comp_def)
-  apply (subst if_P inv_o_simp1 trans[OF comp_apply[symmetric] Pmap_comp0[THEN fun_cong]], (rule valid_Pmap bij_imp_bij_inv supp_inv_bound | assumption)+)+
-  apply (unfold trans[OF Pmap_id0[THEN fun_cong] id_apply])
-  apply (unfold Pmap_def case_prod_beta snd_conv compSS_FType_def)
-
-  apply (subst trans[OF comp_apply[symmetric] FTerm_pre.map_Sb_strong(1)[THEN fun_cong]])
-  apply (assumption | rule cmin1 cmin2 card_of_Card_order FTerm_pre.SSupp_Inj_bound | erule ordLess_ordLeq_trans)+
-  apply (unfold id_o o_id inv_o_simp2)
-  apply (subst FType.vvsubst_permute, (assumption | rule cmin1 cmin2 card_of_Card_order FTerm_pre.SSupp_Inj_bound | erule ordLess_ordLeq_trans)+)
-  apply (unfold comp_def BNF_Composition.id_bnf_def inv_simp2 id_def)
-  apply (rule refl)
-  done
-
-ML \<open>
-val nvars: int = 2
-
-val parameters = {
-  P = @{typ "('tv::var, 'v::var) P"},
-  Pmap = @{term "Pmap :: _ \<Rightarrow> _ \<Rightarrow> _ \<Rightarrow> ('tv::var, 'v::var) P"},
-  PFVarss = [
-    @{term "PFVars_1 :: ('tv::var, 'v::var) P \<Rightarrow> _"},
-    @{term "PFVars_2 :: ('tv::var, 'v::var) P \<Rightarrow> _"}
-  ],
-  avoiding_sets = [@{term "{} :: 'tv::var set"}, @{term "{} :: 'v::var set"}],
-  min_bound = true,
-  validity = SOME {
-    pred = @{term "valid_P :: ('tv::var, 'v::var) P \<Rightarrow> _"},
-    valid_Pmap = fn ctxt => HEADGOAL (resolve_tac ctxt @{thms valid_Pmap} THEN_ALL_NEW assume_tac ctxt)
-  },
-  axioms = {
-    Pmap_id0 = fn ctxt => EVERY1 [
-      resolve_tac ctxt [trans],
-      resolve_tac ctxt @{thms fun_cong[OF Pmap_id0]},
-      resolve_tac ctxt @{thms id_apply}
-    ],
-    Pmap_comp0 = fn ctxt => resolve_tac ctxt @{thms fun_cong[OF Pmap_comp0[symmetric]]} 1 THEN REPEAT_DETERM (assume_tac ctxt 1),
-    Pmap_cong_id = fn ctxt => resolve_tac ctxt @{thms Pmap_cong_id} 1 THEN REPEAT_DETERM (assume_tac ctxt 1 ORELSE Goal.assume_rule_tac ctxt 1),
-    PFVars_Pmaps = replicate nvars (fn ctxt => resolve_tac ctxt @{thms PFVars_Pmaps} 1 THEN REPEAT_DETERM (assume_tac ctxt 1)),
-    small_PFVarss = replicate nvars (fn ctxt => resolve_tac ctxt @{thms small_PFVarss} 1 THEN assume_tac ctxt 1),
-    small_avoiding_sets = replicate nvars (fn ctxt => HEADGOAL (resolve_tac ctxt @{thms cmin_greater}
-      THEN_ALL_NEW resolve_tac ctxt @{thms card_of_Card_order emp_bound}))
-  }
-} : (Proof.context -> tactic) MRBNF_Recursor.parameter;
-\<close>
-
-ML \<open>
-val fp_res = the (MRBNF_FP_Def_Sugar.fp_result_of @{context} "BMV_Fixpoint.FTerm")
-val quot = hd (#quotient_fps fp_res);
-val vars = map TVar (rev (Term.add_tvarsT (#T quot) []));
-\<close>
-
-ML \<open>
-val model = MRBNF_Recursor.mk_quotient_model quot (vars ~~ [@{typ "'tv::var"}, @{typ "'v::var"}]) [] {
-  binding = @{binding "tvsubst_FTerm"},
-  Uctor = @{term "Uctor :: _ \<Rightarrow> ('tv::var, 'v::var) P \<Rightarrow> _"},
-  validity = NONE,
-  axioms = {
-    FVars_subsets = [
-      fn ctxt => EVERY1 [
-        K (Local_Defs.unfold0_tac ctxt @{thms Un_empty_right}),
-        resolve_tac ctxt @{thms FTVars_subset},
-        REPEAT_DETERM o assume_tac ctxt,
-        Goal.assume_rule_tac ctxt
-      ],
-      fn ctxt => EVERY1 [
-        K (Local_Defs.unfold0_tac ctxt @{thms Un_empty_right}),
-        resolve_tac ctxt @{thms FVars_subset},
-        REPEAT_DETERM o assume_tac ctxt,
-        Goal.assume_rule_tac ctxt
-      ]
-    ],
-    permute_Uctor = fn ctxt => HEADGOAL (resolve_tac ctxt @{thms permute_Uctor} THEN_ALL_NEW assume_tac ctxt)
-  }
-}
-\<close>
-
-local_setup \<open>fn lthy =>
-let
-  val qualify = I
-  val (ress, lthy) = MRBNF_Recursor.create_binding_recursor qualify fp_res parameters [model] lthy
-
-  val notes =
-    [ ("rec_Uctor", map (Local_Defs.unfold0 lthy @{thms Un_empty_right} o #rec_Uctor) ress)
-    ] |> (map (fn (thmN, thms) =>
-      ((Binding.qualify true "FTerm" (Binding.name thmN), []), [(thms, [])])
-    ));
-  val (_, lthy) = Local_Theory.notes notes lthy
-  val _ = @{print} ress
-in lthy end
-\<close>
-print_theorems
-
-definition tvsubst_FTerm :: "('v \<Rightarrow> ('tv::var, 'v::var) FTerm) \<Rightarrow> ('tv \<Rightarrow> 'tv FType) \<Rightarrow> ('tv, 'v) FTerm \<Rightarrow> ('tv, 'v) FTerm" where
-  "tvsubst_FTerm f1 f2 t \<equiv> ff0_tvsubst_FTerm t (f1, f2)"
+*)
 
 type_synonym ('tv, 'v) U1_pre = "('tv, 'v, 'tv, 'v, ('tv, 'v) FTerm, ('tv, 'v) FTerm) FTerm_pre"
 
@@ -929,54 +456,261 @@ lemma eta_set_empties:
     done
   done
 
-lemma tvsubst_VVr:
-  assumes
-    "|SSupp_FTerm f1| <o cmin |UNIV::'tv set| |UNIV::'v set|"
-    "|SSupp_FType f2| <o cmin |UNIV::'tv set| |UNIV::'v set|"
-  shows "tvsubst_FTerm f1 f2 (VVr a :: ('tv::var, 'v::var) FTerm) = f1 a"
-  apply (unfold tvsubst_FTerm_def VVr_def comp_def)
+lemmas Cinfinite_UNIV = conjI[OF FTerm_pre.UNIV_cinfinite card_of_Card_order]
+lemmas Cinfinite_card = cmin_Cinfinite[OF Cinfinite_UNIV Cinfinite_UNIV]
+lemmas regularCard_card = cmin_regularCard[OF FTerm_pre.var_regular FTerm_pre.var_regular Cinfinite_UNIV Cinfinite_UNIV]
+lemmas Un_bound = regularCard_Un[OF conjunct2[OF Cinfinite_card] conjunct1[OF Cinfinite_card] regularCard_card]
+lemmas UN_bound = regularCard_UNION[OF conjunct2[OF Cinfinite_card] conjunct1[OF Cinfinite_card] regularCard_card]
+
+context
+  fixes f1::"'var::var \<Rightarrow> ('tyvar::var, 'var) FTerm" and f2::"'tyvar \<Rightarrow> 'tyvar FType"
+  assumes f_prems: "|SSupp VVr f1| <o cmin |UNIV::'tyvar set| |UNIV::'var set|"
+    "|SSupp TyVar f2| <o cmin |UNIV::'tyvar set| |UNIV::'var set|"
+begin
+
+interpretation tvsubst: QREC_cmin_fixed_FTerm "IImsupp_FTerm1 f1 \<union> (SSupp TyVar f2 \<union> IImsupp TyVar FVars_FType f2)"
+  "IImsupp_FTerm2 f1" "\<lambda>y. if isVVr (FTerm_ctor (map_FTerm_pre id id id id fst fst y)) then
+    f1 (asVVr (FTerm_ctor (map_FTerm_pre id id id id fst fst y)))
+  else FTerm_ctor (Sb_FTerm_pre id f2 (map_FTerm_pre id id id id snd snd y))"
+  apply unfold_locales
+
+      apply (((unfold IImsupp_def)[1]), (rule Un_bound UN_bound f_prems card_of_Card_order FTerm.FVars_bd_UNIVs FType.FVars_bd_UNIVs cmin_greater
+        var_class.UN_bound f_prems[THEN ordLess_ordLeq_trans] cmin1 cmin2
+        )+)+
+
+  subgoal for g1 g2 y
+    apply (subst FTerm_pre.map_comp, (assumption | erule ordLess_ordLeq_trans[OF _ cmin1] ordLess_ordLeq_trans[OF _ cmin2] | rule card_of_Card_order supp_id_bound bij_id)+)+
+    apply (unfold Product_Type.snd_comp_map_prod Product_Type.fst_comp_map_prod id_o_commute[of g1] id_o_commute[of g2])
+    apply (subst FTerm_pre.map_comp[symmetric], (assumption | erule ordLess_ordLeq_trans[OF _ cmin1] ordLess_ordLeq_trans[OF _ cmin2] | rule card_of_Card_order supp_id_bound bij_id)+)+
+    apply (subst FTerm.permute_ctor[symmetric] isVVr_permute, (assumption | rule ordLess_ordLeq_trans cmin1 cmin2 card_of_Card_order)+)+
+
+    apply (rule case_split)
+     apply (subst if_P)
+      apply assumption
+     apply (unfold if_P if_not_P)
+     apply (unfold isVVr_def)[1]
+     apply (erule exE)
+    apply (rotate_tac -1)
+     apply (erule subst[OF sym])
+     apply (subst permute_VVr)
+    apply (assumption | rule ordLess_ordLeq_trans cmin1 cmin2 card_of_Card_order)+
+     apply (unfold asVVr_VVr)
+     apply (rule IImsupp_permute_commute[THEN fun_cong, unfolded comp_def])
+          apply (assumption | rule ordLess_ordLeq_trans cmin1 cmin2 card_of_Card_order)+
+      apply (erule Int_subset_empty2)
+      apply (rule subsetI)
+      apply (assumption | erule UnI1 UnI2 | rule UnI1)+
+
+    apply (rule trans)
+    apply (rule FTerm.permute_ctor)
+        apply (assumption | rule ordLess_ordLeq_trans cmin1 cmin2 card_of_Card_order)+
+
+    apply (subst trans[OF comp_apply[symmetric] FTerm_pre.map_Sb_strong(1)[THEN fun_cong]])
+          apply (assumption | erule ordLess_ordLeq_trans[OF _ cmin1] ordLess_ordLeq_trans[OF _ cmin2]
+          | rule card_of_Card_order supp_id_bound bij_id f_prems[THEN ordLess_ordLeq_trans, OF cmin1] f_prems[THEN ordLess_ordLeq_trans, OF cmin2])+
+    apply (unfold0 id_o o_id inv_o_simp2 comp_apply)
+    apply (rule arg_cong[of _ _ FTerm_ctor])
+    apply (rule FTerm_pre.Sb_cong)
+         apply (assumption  | erule ordLess_ordLeq_trans[OF _ cmin1] ordLess_ordLeq_trans[OF _ cmin2]
+        | rule supp_id_bound card_of_Card_order supp_inv_bound SSupp_comp_bound infinite_UNIV FType.SSupp_map_bound
+          f_prems[THEN ordLess_ordLeq_trans, OF cmin1] f_prems[THEN ordLess_ordLeq_trans, OF cmin2]
+        | (unfold comp_assoc)[1])+
+     apply (rule refl)
+    apply (subst (asm) FTerm_pre.map_comp, (assumption | erule ordLess_ordLeq_trans[OF _ cmin1] ordLess_ordLeq_trans[OF _ cmin2] | rule card_of_Card_order supp_id_bound bij_id)+)
+    apply (unfold id_o o_id FTerm_pre.set_Vrs(1)[symmetric])
+    apply (subst (asm) FTerm_pre.set_map, (assumption | erule ordLess_ordLeq_trans[OF _ cmin1] ordLess_ordLeq_trans[OF _ cmin2] | rule card_of_Card_order supp_id_bound bij_id)+)
+    apply (erule imageE)
+    apply hypsubst
+    apply (rule trans[OF comp_apply])
+    apply (unfold inv_simp1)
+    apply (rule trans[OF comp_apply])
+    apply (subst FType.vvsubst_permute, (assumption | rule ordLess_ordLeq_trans cmin1 cmin2 card_of_Card_order)+)
+    apply (rule FType.IImsupp_permute_commute[THEN fun_cong, unfolded comp_def])
+      apply (assumption | rule ordLess_ordLeq_trans cmin1 cmin2 card_of_Card_order)+
+    apply (erule Int_subset_empty2)
+    apply (rule subsetI)
+    apply (rule UnI2)
+    apply (unfold IImsupp_FType_def comp_def SSupp_FType_def tvVVr_tvsubst_FType_def tv\<eta>_FType_tvsubst_FType_def
+      IImsupp_def SSupp_def VVr_def TyVar_def
+    )[1]
+    apply assumption
+    done
+
+  subgoal premises prems
+    apply (rule case_split)
+     apply (subst if_P)
+      apply assumption
+    apply (unfold if_not_P)
+     apply (unfold isVVr_def)[1]
+     apply (erule exE)
+     apply (erule subst[OF sym])
+     apply (unfold asVVr_VVr)
+     apply (rule case_split[of "_ = _"])
+      apply (rule iffD2[OF arg_cong2[OF _ refl, of _ _ "(\<subseteq>)"]])
+       apply (rule arg_cong[of _ _ FTVars])
+       apply assumption
+      apply (rule Un_upper1)
+    apply (rule subsetI)
+     apply (rule UnI2)
+     apply (rule UnI1)
+     apply (unfold IImsupp_def SSupp_def)[1]
+     apply (rule UN_I)
+      apply (rule CollectI)
+      apply assumption
+     apply assumption
+
+    apply (erule thin_rl)
+    apply (subst FTerm_pre.map_Sb[THEN fun_cong, unfolded comp_def, symmetric])
+         apply (rule supp_id_bound bij_id f_prems[THEN ordLess_ordLeq_trans, OF cmin1] f_prems[THEN ordLess_ordLeq_trans, OF cmin2] card_of_Card_order)+
+    apply (unfold FTerm.FVars_ctor)
+    apply (subst FTerm_pre.set_map, (rule supp_id_bound bij_id)+)+
+    apply (unfold image_id image_comp[unfolded comp_def])
+    apply (subst FTerm_pre.set_Sb, (rule supp_id_bound bij_id f_prems[THEN ordLess_ordLeq_trans, OF cmin1] f_prems[THEN ordLess_ordLeq_trans, OF cmin2] card_of_Card_order)+)+
+    apply (rule Un_mono')+
+
+      apply (unfold FTerm_pre.set_Vrs(1))[1]
+      apply (subst FTerm_pre.Vrs_Sb, (rule supp_id_bound bij_id f_prems[THEN ordLess_ordLeq_trans, OF cmin1] f_prems[THEN ordLess_ordLeq_trans, OF cmin2] card_of_Card_order)+)
+      apply (rule subsetI)
+      apply (erule UN_E)
+      apply (rule case_split[of "_ = _", rotated])
+       apply (unfold IImsupp_def SSupp_def)[1]
+       apply (rule UnI2)+
+       apply (rule UN_I)
+        apply (rule CollectI)
+        apply assumption
+       apply assumption
+      apply (rule UnI1)
+      apply (rotate_tac -2)
+      apply (drule iffD1[OF arg_cong2[OF refl, of _ _ "(\<in>)"], rotated])
+       apply (erule arg_cong)
+      apply (unfold FType.Vrs_Inj)
+      apply (drule singletonD)
+      apply hypsubst
+      apply assumption
+
+     apply (rule iffD2[OF arg_cong2[OF refl, of _ _ "(\<subseteq>)"]])
+      apply (rule Diff_Un_disjunct)
+      apply (rule prems)
+     apply (rule Diff_mono[OF _ subset_refl])
+     apply (unfold UN_extend_simps(2))
+    (* REPEAT_DETERM *)
+     apply (rule subset_If)
+      apply (unfold UN_empty')[1]
+      apply (rule empty_subsetI)
+     apply (rule UN_mono[OF subset_refl])
+     apply (rule prems)
+     apply (unfold prod.collapse)
+     apply (erule UnI2 UnI1)
+    (* repeated *)
+     apply (rule subset_If)
+      apply (unfold UN_empty')[1]
+      apply (rule empty_subsetI)
+     apply (rule UN_mono[OF subset_refl])
+     apply (rule prems)
+     apply (unfold prod.collapse)
+     apply (erule UnI2 UnI1)
+    (* END REPEAT_DETERM *)
+    done
+
+
+  subgoal premises prems
+    apply (rule case_split)
+     apply (subst if_P)
+      apply assumption
+    apply (unfold if_not_P)
+     apply (unfold isVVr_def)[1]
+     apply (erule exE)
+     apply (erule subst[OF sym])
+     apply (unfold asVVr_VVr)
+     apply (rule case_split[of "_ = _"])
+      apply (rule iffD2[OF arg_cong2[OF _ refl, of _ _ "(\<subseteq>)"]])
+       apply (rule arg_cong[of _ _ FVars])
+       apply assumption
+      apply (rule Un_upper1)
+    apply (rule subsetI)
+     apply (rule UnI2)
+     apply (unfold IImsupp_def SSupp_def)[1]
+    apply (rule UnI2)
+     apply (rule UN_I)
+      apply (rule CollectI)
+      apply assumption
+     apply assumption
+
+    apply (erule thin_rl)
+    apply (subst FTerm_pre.map_Sb[THEN fun_cong, unfolded comp_def, symmetric])
+         apply (rule supp_id_bound bij_id f_prems[THEN ordLess_ordLeq_trans, OF cmin1] f_prems[THEN ordLess_ordLeq_trans, OF cmin2] card_of_Card_order)+
+    apply (unfold FTerm.FVars_ctor)
+    apply (subst FTerm_pre.set_map, (rule supp_id_bound bij_id)+)+
+    apply (unfold image_id image_comp[unfolded comp_def])
+    apply (subst FTerm_pre.set_Sb, (rule supp_id_bound bij_id f_prems[THEN ordLess_ordLeq_trans, OF cmin1] f_prems[THEN ordLess_ordLeq_trans, OF cmin2] card_of_Card_order)+)+
+    apply (rule Un_mono')+
+
+      apply (unfold FTerm_pre.set_Vrs(2))[1]
+      apply (subst FTerm_pre.Vrs_Sb, (rule supp_id_bound bij_id f_prems[THEN ordLess_ordLeq_trans, OF cmin1] f_prems[THEN ordLess_ordLeq_trans, OF cmin2] card_of_Card_order)+)
+      apply (unfold image_id)
+      apply (rule Un_upper1)
+
+     apply (rule iffD2[OF arg_cong2[OF refl, of _ _ "(\<subseteq>)"]])
+      apply (rule Diff_Un_disjunct)
+      apply (rule prems)
+     apply (rule Diff_mono[OF _ subset_refl])
+     apply (unfold UN_extend_simps(2))
+    (* REPEAT_DETERM *)
+     apply (rule subset_If)
+      apply (unfold UN_empty')[1]
+      apply (rule empty_subsetI)
+     apply (rule UN_mono[OF subset_refl])
+     apply (rule prems)
+     apply (unfold prod.collapse)
+     apply (erule UnI2 UnI1)
+    (* repeated *)
+     apply (rule subset_If)
+      apply (unfold UN_empty')[1]
+      apply (rule empty_subsetI)
+     apply (rule UN_mono[OF subset_refl])
+     apply (rule prems)
+     apply (unfold prod.collapse)
+     apply (erule UnI2 UnI1)
+    (* END REPEAT_DETERM *)
+    done
+  done
+
+definition "tvsubst_FTerm = tvsubst.REC_FTerm"
+
+lemma tvsubst_VVr: "tvsubst_FTerm (VVr a) = f1 a"
+  apply (unfold VVr_def comp_def)
+  apply (unfold tvsubst_FTerm_def)
   apply (rule trans)
-   apply (rule FTerm.rec_Uctor)
-      apply (unfold valid_P_def prod.case)
-      apply (rule conjI assms)+
-     apply (unfold eta_set_empties noclash_FTerm_def Uctor_def Un_empty prod.case)
+   apply (rule tvsubst.REC_ctor)
+     apply (unfold eta_set_empties noclash_FTerm_def)
      apply (rule Int_empty_left conjI)+
   apply (subst FTerm_pre.map_comp, (rule supp_id_bound bij_id)+)+
-  apply (unfold id_o o_id comp_def[of fst] fst_conv id_def[symmetric] FTerm_pre.map_id)
-  apply (rule trans)
-   apply (rule if_P)
-   apply (unfold isVVr_def VVr_def comp_def )
+  apply (unfold id_o o_id comp_def[of fst] fst_conv id_def[symmetric] FTerm_pre.map_id
+      VVr_def[THEN meta_eq_to_obj_eq, THEN fun_cong, unfolded comp_def, symmetric] asVVr_VVr
+      )
+  apply (subst if_P)
+   apply (unfold isVVr_def)
    apply (rule exI)
    apply (rule refl)
-  apply (unfold meta_eq_to_obj_eq[OF VVr_def, THEN fun_cong, unfolded comp_def, symmetric] asVVr_VVr)
   apply (rule refl)
   done
 
-lemma tvsubst_FTerm_no_is_VVr:
-  fixes x::"('tv::var, 'v::var) U1_pre"
-  assumes f_prems: "|SSupp_FTerm f1| <o cmin |UNIV::'tv set| |UNIV::'v set|" "|SSupp_FType f2| <o cmin |UNIV::'tv set| |UNIV::'v set|"
-    and empty_prems: "set3_FTerm_pre x \<inter> (IImsupp_FTerm1 f1 \<union> IImsupp_FType f2) = {}" "set4_FTerm_pre x \<inter> IImsupp_FTerm2 f1 = {}"
-    and noclash: "noclash_FTerm x"
-    and VVr_prems: "\<not>isVVr (FTerm_ctor x)"
-  shows
-    "tvsubst_FTerm f1 f2 (FTerm_ctor x) = FTerm_ctor (Sb_FTerm_pre id f2 (map_FTerm_pre id id id id (tvsubst_FTerm f1 f2) (tvsubst_FTerm f1 f2) x))"
+lemma tvsubst_FTerm_not_is_VVr:
+  assumes empty_prems: "set3_FTerm_pre x \<inter> (IImsupp_FTerm1 f1 \<union> (SSupp TyVar f2 \<union> IImsupp TyVar FVars_FType f2)) = {}" "set4_FTerm_pre x \<inter> IImsupp_FTerm2 f1 = {}"
+  and noclash: "noclash_FTerm x"
+  and VVr_prems: "\<not>isVVr (FTerm_ctor x)"
+  shows "tvsubst_FTerm (FTerm_ctor x) = FTerm_ctor (Sb_FTerm_pre id f2 (map_FTerm_pre id id id id tvsubst_FTerm tvsubst_FTerm x))"
   apply (unfold tvsubst_FTerm_def)
-  apply (subgoal_tac "valid_P (f1, f2)")
-   prefer 2
-   apply (unfold valid_P_def prod.case)[1]
-   apply (rule conjI f_prems)+
   apply (rule trans)
-   apply (rule FTerm.rec_Uctor)
-      apply assumption
-     apply (unfold PFVars_1_def PFVars_2_def prod.case)
-     apply (rule empty_prems noclash)+
-  apply (unfold Uctor_def prod.case)
+   apply (rule tvsubst.REC_ctor)
+     apply (rule assms)+
   apply (subst FTerm_pre.map_comp, (rule supp_id_bound bij_id)+)+
-  apply (unfold id_o o_id comp_def[of fst] fst_conv id_def[symmetric] FTerm_pre.map_id)
-  apply (subst if_not_P, rule VVr_prems)+
-  apply (unfold comp_def snd_conv if_P)
-  apply (rule refl)
+  apply (unfold id_o o_id comp_def[of fst] comp_def[of snd] snd_conv fst_conv id_def[symmetric] FTerm_pre.map_id)
+  apply (rule if_not_P)
+  apply (rule assms)
   done
+
+end
 
 (* Sugar theorems for substitution *)
 definition Var :: "'v \<Rightarrow> ('tv::var, 'v::var) FTerm" where
@@ -992,20 +726,20 @@ definition TyLam :: "'tv \<Rightarrow> ('tv, 'v) FTerm \<Rightarrow> ('tv::var, 
 
 lemma FTerm_subst:
   fixes f1::"'v \<Rightarrow> ('tv::var, 'v::var) FTerm" and f2::"'tv \<Rightarrow> 'tv FType"
-  assumes "|SSupp_FTerm f1| <o cmin |UNIV::'tv set| |UNIV::'v set|" "|SSupp_FType f2| <o cmin |UNIV::'tv set| |UNIV::'v set|"
+  assumes "|SSupp VVr f1| <o cmin |UNIV::'tv set| |UNIV::'v set|" "|SSupp TyVar f2| <o cmin |UNIV::'tv set| |UNIV::'v set|"
   shows
     "tvsubst_FTerm f1 f2 (Var x) = f1 x"
     "tvsubst_FTerm f1 f2 (App t1 t2) = App (tvsubst_FTerm f1 f2 t1) (tvsubst_FTerm f1 f2 t2)"
     "tvsubst_FTerm f1 f2 (TyApp t T) = TyApp (tvsubst_FTerm f1 f2 t) (tvsubst_FType f2 T)"
     "x \<notin> IImsupp_FTerm2 f1 \<Longrightarrow> tvsubst_FTerm f1 f2 (Lam x T t) = Lam x (tvsubst_FType f2 T) (tvsubst_FTerm f1 f2 t)"
-    "a \<notin> IImsupp_FTerm1 f1 \<union> IImsupp_FType f2 \<Longrightarrow> tvsubst_FTerm f1 f2 (TyLam a t) = TyLam a (tvsubst_FTerm f1 f2 t)"
+    "a \<notin> IImsupp_FTerm1 f1 \<union> (SSupp TyVar f2 \<union> IImsupp TyVar FVars_FType f2) \<Longrightarrow> tvsubst_FTerm f1 f2 (TyLam a t) = TyLam a (tvsubst_FTerm f1 f2 t)"
       apply (unfold Var_def App_def TyApp_def Lam_def TyLam_def)
       apply (unfold meta_eq_to_obj_eq[OF VVr_def, THEN fun_cong, unfolded comp_def, symmetric])
       apply (rule tvsubst_VVr)
        apply (rule assms)+
 
      apply (rule trans)
-      apply (rule tvsubst_FTerm_no_is_VVr)
+      apply (rule tvsubst_FTerm_not_is_VVr)
            apply (rule assms)+
          apply (unfold set3_FTerm_pre_def sum.set_map prod.set_map UN_empty2 Un_empty_left Un_empty_right UN_singleton comp_def
       Abs_FTerm_pre_inverse[OF UNIV_I] sum_set_simps UN_single UN_empty set4_FTerm_pre_def noclash_FTerm_def
@@ -1026,7 +760,7 @@ lemma FTerm_subst:
      apply (rule refl)
 
     apply (rule trans)
-     apply (rule tvsubst_FTerm_no_is_VVr)
+     apply (rule tvsubst_FTerm_not_is_VVr)
           apply (rule assms)+
         apply (unfold set3_FTerm_pre_def sum.set_map prod.set_map UN_empty2 Un_empty_left Un_empty_right UN_singleton comp_def
       Abs_FTerm_pre_inverse[OF UNIV_I] sum_set_simps UN_single UN_empty set4_FTerm_pre_def noclash_FTerm_def
@@ -1048,7 +782,7 @@ lemma FTerm_subst:
     apply (rule refl)
 
    apply (rule trans)
-    apply (rule tvsubst_FTerm_no_is_VVr)
+    apply (rule tvsubst_FTerm_not_is_VVr)
          apply (rule assms)+
        apply (unfold set2_FTerm_pre_def set6_FTerm_pre_def set3_FTerm_pre_def sum.set_map prod.set_map UN_empty2 Un_empty_left Un_empty_right UN_singleton comp_def
       Abs_FTerm_pre_inverse[OF UNIV_I] sum_set_simps UN_single UN_empty set4_FTerm_pre_def noclash_FTerm_def prod_set_simps
@@ -1070,7 +804,7 @@ lemma FTerm_subst:
    apply (rule refl)
 
   apply (rule trans)
-   apply (rule tvsubst_FTerm_no_is_VVr)
+   apply (rule tvsubst_FTerm_not_is_VVr)
         apply (rule assms)+
       apply (unfold set2_FTerm_pre_def set6_FTerm_pre_def set3_FTerm_pre_def sum.set_map prod.set_map UN_empty2 Un_empty_left Un_empty_right UN_singleton comp_def
       Abs_FTerm_pre_inverse[OF UNIV_I] sum_set_simps UN_single UN_empty set4_FTerm_pre_def noclash_FTerm_def prod_set_simps
